ln/STLC_Ref_Soundness_OmniBig.v
@@ -6,462 +6,129 @@
 (** The proof is explained in the Omni-Semantics paper (TOPLAS'23).
      http://www.chargueraud.org/research/2022/omnisemantics/omnisemantics.pdf *)
 
+
 Set Implicit Arguments.
-Set Implicit Arguments.
-From TLC Require Import LibLN LibNat.
-Require Import STLC_Ref_Definitions STLC_Ref_Infrastructure.
+Require Import STLC_Ref_Soundness_Common.
+Implicit Types Y : phi.
 
+(* ********************************************************************** *)
+(** * Definition of Co-Omni-Big-Step Semantics *)
 
+(** The coinductive omni-big-step judgment [omnibig c P], where [P] is a
+    postcondition, asserts that all possibly evaluations of [c] are never stuck
+    and can only reach final configurations that satisfy [P].
+    The judgment is coinductive: it captures partial correctness.
+    Technically, this judgment follows the pretty-big-step presentation:
+    each rule evaluates exactly one subterm, replacing this subterm with a value. *)
 
-Hint Constructors typing.
-
-(** Typing is preserved by weakening. *)
-
-Lemma typing_weaken : forall G E F Y t T,
-   (E & G) ! Y |= t ~: T ->
-   ok (E & F & G) ->
-   (E & F & G) ! Y |= t ~: T.
-Proof.
-  introv Typ. gen_eq H: (E & G). gen G.
-  induction Typ; introv EQ Ok; subst.
-  apply* typing_var. apply* binds_weaken.
-  apply_fresh* typing_abs as y. apply_ih_bind* H0.
-  autos*.
-  autos*.
-  autos*.
-  autos*.
-  autos*.
-  autos*.
-  autos*.
-  autos*.
-Qed.
-
-(** Typing is preserved by substitution. *)
-
-Lemma typing_subst : forall F E Y t T z u U,
-  (E & z ~ U & F) ! Y |= t ~: T ->
-  E ! Y |= u ~: U ->
-  (E & F) ! Y |= [z ~> u]t ~: T.
-Proof.
-  introv Typt Typu. gen_eq G: (E & z ~ U & F). gen F.
-  induction Typt; introv Equ; subst; simpl subst.
-  case_var.
-    binds_get H0. apply_empty* typing_weaken.
-    binds_cases H0; apply* typing_var.
-  apply_fresh typing_abs as y.
-   rewrite* subst_open_var. apply_ih_bind* H0.
-  autos*.
-  autos*.
-  autos*.
-  autos*.
-  autos*.
-  autos*.
-  autos*.
-  autos*.
-Qed.
-
-(** Typing is preserved by an extension of store typing. *)
-
-Lemma typing_stability : forall Y E Y' t T,
-  E ! Y |= t ~: T ->
-  extends Y Y' ->
-  E ! Y' |= t ~: T.
-Proof.
-  introv Typ Ext. induction* Typ.
-Qed.
-
-Hint Resolve typing_stability.
-
-(** Store typing preserved by allocation of a well-typed term. *)
-
-Lemma sto_typing_push : forall Y mu l t T,
-  Y |== mu ->
-  empty ! Y |= t ~: T ->
-  l # mu -> l # Y ->
-  (Y & l ~ T) |== (mu & l ~ t).
-Proof.
-  unfold sto_typing. introv [StoOk [Dom Ext]]. splits 3.
-    auto.
-    intros l0 Fr. simpl_dom. lets: (Dom l0).
-      asserts* Fr2: (l <> l0). asserts* Fr3: (l0 # Y). auto.
-    intros l' T' Has. binds_cases Has.
-      destruct (Ext _ _ B) as [t' [Hast' Typt']].
-       exists* t'.
-      subst. exists* t.
-Qed.
-
-
-
-(** Omni-Small-Step semantics [omnismall c Y]. *)
-
-CoInductive omnismall : conf -> (conf->Prop) -> Prop :=
-  | omnismall_beta : forall mu t1 t2 P,
+CoInductive coomnibig : conf -> (conf->Prop) -> Prop :=
+  | coomnibig_val : forall c P,
+      value (fst c) ->
+      P c ->
+      coomnibig c P
+  | coomnibig_beta : forall mu t1 t2 P,
       sto_ok mu ->
       term (trm_abs t1) ->
       value t2 ->
-      P (t1 ^^ t2, mu) ->
-      omnismall (trm_app (trm_abs t1) t2, mu) P
-  | omnismall_ref : forall mu t1 P,
+      coomnibig (t1 ^^ t2, mu) P ->
+      coomnibig (trm_app (trm_abs t1) t2, mu) P
+  | coomnibig_rand : forall mu n P,
+      (forall m, 0 <= m < max n 1 -> P ((trm_int m), mu)) ->
+      coomnibig (trm_rand (trm_int n), mu) P
+  | coomnibig_ref : forall mu t1 P,
       sto_ok mu ->
       value t1 ->
-      (forall l, l # mu -> P (trm_loc l, (mu & l ~ t1))) ->
-      omnismall (trm_ref t1, mu) P
-  | omnismall_get : forall mu l t P,
+      (forall l, l # mu ->
+        P (trm_loc l, (mu & l ~ t1))) ->
+      coomnibig (trm_ref t1, mu) P
+  | coomnibig_get : forall mu l t P,
       sto_ok mu ->
       binds l t mu ->
       P (t, mu) ->
-      omnismall (trm_get (trm_loc l), mu) P
-  | omnismall_set : forall mu l t2 P,
+      coomnibig (trm_get (trm_loc l), mu) P
+  | coomnibig_set : forall mu l t2 P,
       sto_ok mu ->
       value t2 ->
       P (trm_unit, mu & l ~ t2) ->
-      omnismall (trm_set (trm_loc l) t2, mu) P
-  | omnismall_rand : forall mu n P,
-      (forall m, 0 <= m < max n 1 -> P ((trm_int m), mu)) ->
-      omnismall (trm_rand (trm_int n), mu) P
+      coomnibig (trm_set (trm_loc l) t2, mu) P
 
-  | omnismall_app_1 : forall mu t1 t2 P1 P,
-      omnismall (t1, mu) P1 ->
-      (forall t1' mu', P1 (t1',mu') -> P (trm_app t1' t2, mu')) ->
-      omnismall (trm_app t1 t2, mu) P
-  | omnismall_app_2 : forall mu t1 t2 P1 P,
+  | coomnibig_app_1 : forall mu t1 t2 P1 P,
+      ~ value t1 ->
+      coomnibig (t1, mu) P1 ->
+      (forall t1' mu', P1 (t1',mu') -> coomnibig (trm_app t1' t2, mu') P) ->
+      coomnibig (trm_app t1 t2, mu) P
+  | coomnibig_app_2 : forall mu t1 t2 P1 P,
       value t1 ->
-      omnismall (t2, mu) P1 ->
-      (forall t2' mu', P1 (t2',mu') -> P (trm_app t1 t2', mu')) ->
-      omnismall (trm_app t1 t2, mu) P
-  | omnismall_ref_1 : forall mu t1 P1 P,
-      omnismall (t1, mu) P1 ->
-      (forall t1' mu', P1 (t1',mu') -> P (trm_ref t1', mu')) ->
-      omnismall (trm_ref t1, mu) P
-  | omnismall_get_1 : forall mu t1 P1 P,
-      omnismall (t1, mu) P1 ->
-      (forall t1' mu', P1 (t1',mu') -> P (trm_get t1', mu')) ->
-      omnismall (trm_get t1, mu) P
-  | omnismall_set_1 : forall mu t1 t2 P1 P,
-      omnismall (t1, mu) P1 ->
-      (forall t1' mu', P1 (t1',mu') -> P (trm_set t1' t2, mu')) ->
-      omnismall (trm_set t1 t2, mu) P
-  | omnismall_set_2 : forall mu t1 t2 P1 P,
+      ~ value t2 ->
+      coomnibig (t2, mu) P1 ->
+      (forall t2' mu', P1 (t2',mu') -> coomnibig (trm_app t1 t2', mu') P) ->
+      coomnibig (trm_app t1 t2, mu) P
+  | coomnibig_ref_1 : forall mu t1 P1 P,
+      ~ value t1 ->
+      coomnibig (t1, mu) P1 ->
+      (forall t1' mu', P1 (t1',mu') -> coomnibig (trm_ref t1', mu') P) ->
+      coomnibig (trm_ref t1, mu) P
+  | coomnibig_get_1 : forall mu t1 P1 P,
+      coomnibig (t1, mu) P1 ->
+      (forall t1' mu', P1 (t1',mu') -> coomnibig (trm_get t1', mu') P) ->
+      coomnibig (trm_get t1, mu) P
+  | coomnibig_set_1 : forall mu t1 t2 P1 P,
+      ~ value t1 ->
+      coomnibig (t1, mu) P1 ->
+      (forall t1' mu', P1 (t1',mu') -> coomnibig (trm_set t1' t2, mu') P) ->
+      coomnibig (trm_set t1 t2, mu) P
+  | coomnibig_set_2 : forall mu t1 t2 P1 P,
       value t1 ->
-      omnismall (t2, mu) P1 ->
-      (forall t2' mu', P1 (t2',mu') -> P (trm_set t1 t2', mu')) ->
-      omnismall (trm_set t1 t2, mu) P
-  | omnismall_rand_1 : forall mu t1 P1 P,
-      omnismall (t1, mu) P1 ->
-      (forall t1' mu', P1 (t1',mu') -> P (trm_rand t1', mu')) ->
-      omnismall (trm_rand t1, mu) P.
+      ~ value t2 ->
+      coomnibig (t2, mu) P1 ->
+      (forall t2' mu', P1 (t2',mu') -> coomnibig (trm_set t1 t2', mu') P) ->
+      coomnibig (trm_set t1 t2, mu) P
+  | coomnibig_rand_1 : forall mu t1 P1 P,
+      ~ value t1 ->
+      coomnibig (t1, mu) P1 ->
+      (forall t1' mu', P1 (t1',mu') -> coomnibig (trm_rand t1', mu') P) ->
+      coomnibig (trm_rand t1, mu) P.
+
+(** The folder '/omni' of this repository contains a proof establishing
+    that omni-big-step entails the safety property expressed in small-step.
+    This proof is explained near the end of the chapter "Triples" in the
+    course "Separation Logic Foundations" of the Software Foundations series. *)
 
 
-Hint Constructors omnismall typing.
+(* ********************************************************************** *)
+(** * Statement *)
 
-(** Postcondition associated with a type *)
+(** Postcondition associated with a well-typed configuration;
+    in big-step, postconditions are restricted to final configurations *)
 
 Definition post (Y:phi) (T:typ) : conf->Prop :=
   fun '(t,mu) =>
     exists Y', extends Y Y'
              /\ Y' |== mu
+             /\ value t
              /\ empty ! Y' |= t ~: T.
 
-Lemma post_current : forall Y mu t T,
+(** Goal is to prove coomnibig-soundness: well-typed configurations
+    can only reach final states satisfying the postcondition
+    associated with their types. *)
+
+Definition coomnibig_soundness := forall mu t Y T,
   Y |== mu ->
   empty ! Y |= t ~: T ->
-  post Y T (t,mu).
-Proof using.
-  introv HS HT. exists Y. splits*.
-Qed.
-
-Hint Resolve post_current.
-
-(** Soundness proof *)
-
-Definition omnismall_soundness :=
-  forall mu t Y T,
-  Y |== mu ->
-  empty ! Y |= t ~: T ->
-  value t \/ omnismall (t,mu) (post Y T).
-
-Ltac sound_ctx E :=
-  let Y' := fresh "Y'" in
-  applys* E; try (introv (Y'&?&?&?); exists* Y').
-
-Lemma omnismall_soundness_induction :
-  omnismall_soundness.
-Proof using.
-  introv HS HT. gen_eq E: (@empty typ). gen mu.
-  induction HT; intros; subst; try solve [left* ].
-  { false* binds_empty_inv. }
-  { left*. constructors.
-    { applys term_abs L. intros x Hx. forwards*: H x. } }
-  { right. forwards* [Val1|HR1]: IHHT1.
-    { forwards* [Val2|HR2]: IHHT2.
-      { inversions HT1; inversions Val1. applys* omnismall_beta.
-        { applys* post_current.
-          pick_fresh x. rewrite* (@subst_intro x).
-          apply_empty* typing_subst. } }
-      { sound_ctx omnismall_app_2. } }
-    { sound_ctx omnismall_app_1. } }
-  { right. forwards* [Val1|HR1]: IHHT.
-    { applys* omnismall_ref. intros l Hl. exists (Y & l ~ T).
-      lets: (proj32 HS) Hl. splits*. { applys* sto_typing_push. } }
-    { sound_ctx omnismall_ref_1. } }
-  { right. forwards* [Val1|HR1]: IHHT.
-    { inverts HT; inverts Val1. destruct~ ((proj33 HS) l0 T) as [t [Hast Typt]].
-      applys* omnismall_get. }
-    { sound_ctx omnismall_get_1. } }
-  { right. forwards* [Val1|HR1]: IHHT1.
-    { forwards* [Val2|HR2]: IHHT2.
-      { inverts HT1; inverts Val1. destruct~ ((proj33 HS) l0 T) as [t [Hast Typt]].
-        applys* omnismall_set. exists Y.
-        destruct HS as [StoOk [Dom Map]]. splits*.
-        { splits*. intros l T' HB. tests: (l = l0).
-          { exists t2. rewrites* (>> binds_functional T' T HB). }
-          { destruct (Map _ _ HB) as [t' [Has Typ]]. exists* t'. } } }
-      { sound_ctx omnismall_set_2. } }
-    { sound_ctx omnismall_set_1. } }
-  { right. forwards* [Val1|HR1]: IHHT.
-    { inverts HT; inverts Val1. applys* omnismall_rand. }
-    { sound_ctx omnismall_rand_1. } }
-Qed.
-
-(** We next give a generic proof that [omnismall_soundness_induction]
-    entails [type soundness], under the assumption that the omni-small-step
-    judgment admits the expected postretation w.r.t. the standard
-    small-step judgment. *)
-
-Parameter omnismall_characterization : forall c P,
-  omnismall c P <->
-    (   (exists c', c --> c')
-     /\ (forall c', c --> c' -> P c')).
-
-(** Statement of the soundness property using omni-small-step. *)
-
-Lemma soundness_of_omnismall_soundness :
-  omnismall_soundness ->
-  type_soundness.
-Proof using.
-  introv Sou. intros (t,mu) (Y&T&HT&HY). introv HR.
-  gen_eq c: (t,mu). gen t mu Y T. induction HR; intros; subst.
-  { intros. forwards [HV|M]: Sou HY HT.
-    { left*. }
-    { right. rewrite* omnismall_characterization in M. } }
-  { lets [HV|M]: Sou HY HT.
-    { inverts HV; inverts H. }
-    { rewrite omnismall_characterization in M. destruct M as (M1&M2).
-      specializes M2 H. destruct c2 as (t2,mu2).
-      destruct M2 as (Y'&EY'&HY'&HT'). applys* IHHR HT'. } }
-Qed.
-
-
-
-
-
-(** Value or variable predicate---for A-normal form. *)
-
-Definition val_or_var (t:trm) : Prop :=
-     value t
-  \/ (exists x, t = trm_fvar x).
-
-(** Typing relation *)
-
-Reserved Notation "E ! Y |= t ~: T" (at level 69).
-
-Inductive typing : env -> phi -> trm -> typ -> Prop :=
-  | typing_var : forall E Y x T,
-      ok E ->
-      binds x T E ->
-      E ! Y |= (trm_fvar x) ~: T
-  | typing_abs : forall L E Y U T t1,
-      (forall x, x \notin L -> (E & x ~ U) ! Y  |= t1 ^ x ~: T) ->
-      E ! Y |= (trm_abs t1) ~: (typ_arrow U T)
-  | typing_app : forall T1 T2 E Y t1 t2,
-      val_or_var t1 ->
-      E ! Y |= t1 ~: (typ_arrow T1 T2) -> E ! Y  |= t2 ~: T1 ->
-      E ! Y  |= (trm_app t1 t2) ~: T2
-  | typing_unit : forall E Y,
-      ok E ->
-      E ! Y |= trm_unit ~: typ_unit
-  | typing_int : forall E Y n,
-      ok E ->
-      E ! Y |= (trm_int n) ~: typ_int
-  | typing_loc : forall E Y l T,
-      ok E ->
-      binds l T Y ->
-      E ! Y |= (trm_loc l) ~: (typ_ref T)
-  | typing_ref : forall E Y t1 T,
-      val_or_var t1 ->
-      E ! Y |= t1 ~: T ->
-      E ! Y |= (trm_ref t1) ~: (typ_ref T)
-  | typing_get : forall E Y t1 T,
-      val_or_var t1 ->
-      E ! Y |= t1 ~: (typ_ref T) ->
-      E ! Y |= (trm_get t1) ~: T
-  | typing_set : forall E Y t1 t2 T,
-      val_or_var t1 ->
-      val_or_var t2 ->
-      E ! Y |= t1 ~: (typ_ref T) ->
-      E ! Y |= t2 ~: T ->
-      E ! Y |= (trm_set t1 t2) ~: typ_unit
-  | typing_rand : forall E Y t1,
-      val_or_var t1 ->
-      E ! Y |= t1 ~: typ_int ->
-      E ! Y |= (trm_rand t1) ~: typ_int
-
-where "E ! Y |= t ~: T" := (typing E Y t T).
-
-(** Typing judgment for stores *)
-
-Definition sto_typing Y mu :=
-     sto_ok mu
-  /\ (forall l, l # mu -> l # Y)
-  /\ (forall l T, binds l T Y ->
-        exists t, binds l t mu
-               /\ empty ! Y |= t ~: T).
-
-Notation "Y |== mu" := (sto_typing Y mu) (at level 68).
-
-
-(* ********************************************************************** *)
-(** ** Property of [val_or_var] *)
-
-(** [val_of_var] is stable by substitution. *)
-
-Lemma subst_val_or_var : forall t z u,
-  value u -> val_or_var t -> val_or_var ([z ~> u]t).
-Proof using.
-  introv HT [HV|(x&->)].
-  { left. applys* subst_value. }
-  { simpl. case_var. { left*. } { right*. } }
-Qed.
-
-Hint Extern 1 (val_or_var ([_ ~> _]_)) => apply subst_val_or_var.
-
-
-(** Values and variables don't reduce. *)
-
-Lemma red_val_or_var_inv : forall t mu c,
-  val_or_var t ->
-  (t,mu) --> c ->
-  False.
-Proof using.
-  introv Ht Hc. inverts Ht as.
-  { introv Hv. inverts Hv; inverts Hc. }
-  { introv (x&->). inverts Hc. }
-Qed.
-
-(** Values-or-variables well-typed in the empty contexts are values. *)
-
-Lemma value_of_not_var : forall t S T,
-  typing empty S t T ->
-  val_or_var t ->
-  value t.
-Proof using.
-  introv HT [Hv|(x&->)].
-  { auto. }
-  { inverts HT as. intros K E. false binds_empty_inv E. }
-Qed.
-
-
-
+  coomnibig (t,mu) (post Y T).
 
 
 (* ########################################################### *)
-(* ########################################################### *)
-(* ########################################################### *)
-(** * Weakening, Substitution, and Extension lemmas *)
-
-(** Typing is preserved by weakening. *)
-
-Lemma typing_weaken : forall G E F Y t T,
-   (E & G) ! Y |= t ~: T ->
-   ok (E & F & G) ->
-   (E & F & G) ! Y |= t ~: T.
-Proof.
-  introv Typ. gen_eq H: (E & G). gen G.
-  induction Typ; introv EQ Ok; subst.
-  apply* typing_var. apply* binds_weaken.
-  apply_fresh* typing_abs as y. apply_ih_bind* H0.
-  autos*.
-  autos*.
-  autos*.
-  autos*.
-  autos*.
-  autos*.
-  autos*.
-  autos*.
-Qed.
-
-(** Typing is preserved by substitution. *)
-
-Lemma typing_subst : forall F E Y t T z u U,
-  value u ->
-  (E & z ~ U & F) ! Y |= t ~: T ->
-  E ! Y |= u ~: U ->
-  (E & F) ! Y |= [z ~> u]t ~: T.
-Proof.
-  introv Hu Typt Typu. gen_eq G: (E & z ~ U & F). gen F.
-  induction Typt; introv Equ; subst; simpl subst.
-  case_var.
-    binds_get H0. apply_empty* typing_weaken.
-    binds_cases H0; apply* typing_var.
-  apply_fresh typing_abs as y.
-   rewrite* subst_open_var. apply_ih_bind* H0.
-  autos*.
-  autos*.
-  autos*.
-  autos*.
-  autos*.
-  eauto 9.
-  eauto 9.
-  eauto 9.
-Qed.
-
-(** Typing is preserved by an extension of store typing. *)
-
-Lemma typing_stability : forall Y E Y' t T,
-  E ! Y |= t ~: T ->
-  extends Y Y' ->
-  E ! Y' |= t ~: T.
-Proof.
-  introv Typ Ext. induction* Typ.
-Qed.
-
-Hint Resolve typing_stability.
-
-(** Store typing preserved by allocation of a well-typed term. *)
-
-Lemma sto_typing_push : forall Y mu l t T,
-  Y |== mu ->
-  empty ! Y |= t ~: T ->
-  l # mu -> l # Y ->
-  (Y & l ~ T) |== (mu & l ~ t).
-Proof.
-  unfold sto_typing. introv [StoOk [Dom Ext]]. splits 3.
-    auto.
-    intros l0 Fr. simpl_dom. lets: (Dom l0).
-      asserts* Fr2: (l <> l0). asserts* Fr3: (l0 # Y). auto.
-    intros l' T' Has. binds_cases Has.
-      destruct (Ext _ _ B) as [t' [Hast' Typt']].
-       exists* t'.
-      subst. exists* t.
-Qed.
-
-
-
-
-
-
-(* ########################################################### *)
-(* ########################################################### *)
-(* ########################################################### *)
-(** * Omni-Big-Step Soundness Proof *)
-
-(* ########################################################### *)
-(** ** Entailment on postconditions *)
+(** ** Entailment *)
 
 Definition himpl (H1 H2:conf->Prop) : Prop :=
   forall h, H1 h -> H2 h.
 
 Notation "H1 ==> H2" := (himpl H1 H2) (at level 55).
+
+Lemma himpl_refl : forall H,
+  (H ==> H).
+Proof using. introv M. unfolds* himpl. Qed.
 
 Lemma himpl_trans : forall H2 H1 H3,
   (H1 ==> H2) ->
@@ -469,65 +136,45 @@ Lemma himpl_trans : forall H2 H1 H3,
   (H1 ==> H3).
 Proof using. introv M1 M2. unfolds* himpl. Qed.
 
+(** For technical reasons associated with the guard condition of the
+    coinductive proof, we need to reformulate the soundness statement,
+    by introducing a postcondition [P] that contains [post Y T]. *)
+
+Definition coomnibig_soundness_himpl := forall t mu Y T P,
+  Y |== mu ->
+  empty ! Y |= t ~: T ->
+  (post Y T ==> P) ->
+  coomnibig (t,mu) P.
+
+(** The above statement clearly entails the desired result. *)
+
+Lemma coomnibig_soundness_of_himpl_soundness :
+  coomnibig_soundness_himpl ->
+  coomnibig_soundness.
+Proof using. introv M HS HT. applys* M. applys* himpl_refl. Qed.
+
 
 (* ########################################################### *)
-(** ** Definition of Omni-Big-Step *)
-
-(** Judgment [omnibig c Q]. Here [Q] is a predicate over configurations,
-    but in practice in contains only values. *)
-
-CoInductive coomnibig : conf -> (conf->Prop) -> Prop :=
-  | coomnibig_val : forall c Q,
-      conf_value c ->
-      Q c ->
-      coomnibig c Q
-  | coomnibig_beta : forall mu t1 t2 Q,
-      sto_ok mu ->
-      term (trm_abs t1) ->
-      value t2 ->
-      coomnibig (t1 ^^ t2, mu) Q ->
-      coomnibig (trm_app (trm_abs t1) t2, mu) Q
-  | coomnibig_rand : forall mu n Q,
-      (forall m, 0 <= m < max n 1 -> Q ((trm_int m), mu)) ->
-      coomnibig (trm_rand (trm_int n), mu) Q
-  | coomnibig_ref : forall mu t1 Q,
-      sto_ok mu ->
-      value t1 ->
-      (forall l, l # mu ->
-        Q (trm_loc l, (mu & l ~ t1))) ->
-      coomnibig (trm_ref t1, mu) Q
-  | coomnibig_get : forall mu l t Q,
-      sto_ok mu ->
-      binds l t mu ->
-      Q (t, mu) ->
-      coomnibig (trm_get (trm_loc l), mu) Q
-  | coomnibig_set : forall mu l t2 Q,
-      sto_ok mu ->
-      value t2 ->
-      Q (trm_unit, mu & l ~ t2) ->
-      coomnibig (trm_set (trm_loc l) t2, mu) Q
-  | coomnibig_app_2 : forall mu t1 t2 Q1 Q,
-      value t1 ->
-      ~ value t2 ->
-      coomnibig (t2, mu) Q1 ->
-      (forall t2' mu', Q1 (t2',mu') -> coomnibig (trm_app t1 t2', mu') Q) ->
-      coomnibig (trm_app t1 t2, mu) Q.
+(** ** Lemmas about covariance and extensions *)
 
 (** [coomnibig] is covariant in the postcondition (omni-big-conseqence) *)
 
-Lemma coomnibig_conseq : forall c Q1 Q2,
-  coomnibig c Q1 ->
-  Q1 ==> Q2 ->
+Lemma coomnibig_conseq : forall c P1 Q2,
+  coomnibig c P1 ->
+  P1 ==> Q2 ->
   coomnibig c Q2.
 Proof using.
-  introv M W. unfolds himpl. gen c Q1 Q2. cofix IH.
+  introv M W. unfolds himpl. gen c P1 Q2. cofix IH.
   intros. inverts M; try solve [ constructors* ].
   { applys* coomnibig_get. }
+  { applys* coomnibig_app_1. }
   { applys* coomnibig_app_2. }
+  { applys* coomnibig_ref_1. }
+  { applys* coomnibig_get_1. }
+  { applys* coomnibig_set_1. }
+  { applys* coomnibig_set_2. }
+  { applys* coomnibig_rand_1. }
 Qed.
-
-(** We reuse [post] from the previous section, and
-    add two lemmas. *)
 
 Lemma extends_trans : forall Y2 Y1 Y3,
   extends Y1 Y2 ->
@@ -545,103 +192,63 @@ Qed.
 
 (** Type soundness proof *)
 
-(** Note: if we try to prove directly the statement:
+Ltac auto_star ::= eauto 8.
 
-[[
-    Lemma coomnibig_soundness_coinduction : forall t mu Y T,
-      Y |== mu ->
-      empty ! Y |= t ~: T ->
-      coomnibig (t,mu) (post Y T).
-]]
+Hint Unfold post.
+Hint Constructors value.
 
-  then Cpq's guard checker is not happy because we apply the consequence
-  rule for [coomnibig] needs to be applied before the coinduction hypothesis.
-  Hence, we need to tweak the statement slightly for the coinduction,
-  then derive the desired result. *)
+(** There are some repeated proof patterns for handling evaluation under a context;
+    due to restrictions of the guard condition checker, it is hard to capture
+    those patterns using a lemma, hence we need a tactic to factorize the work. *)
 
-Definition coomnibig_soundness := forall t mu Y T Q,
-  Y |== mu ->
-  empty ! Y |= t ~: T ->
-  (post Y T ==> Q) ->
-  coomnibig (t,mu) Q.
+Ltac sound_ctx E :=
+  let IH := match goal with IH: context [ coomnibig ] |- _ => constr:(IH) end in
+  applys E; try match goal with |- value _ => eauto | |- ~value _ => eauto end;
+  [ applys* IH; try applys himpl_refl
+  | let EY' := fresh "EY'" in
+    introv (Y'&EY'&?&?&?); applys* IH;
+    try (match goal with HQ: post _ _ ==> _ |- _ => applys himpl_trans HQ end;
+         applys post_extends EY') ].
 
-Lemma coomnibig_soundness_coinduction :
-  coomnibig_soundness.
+Lemma coomnibig_soundness_himpl_result :
+  coomnibig_soundness_himpl.
 Proof using.
   unfolds. cofix IH. introv HS HT HQ. inverts HT as.
   { introv HK HT1. false* binds_empty_inv. }
-  { intros L M. applys* coomnibig_val. hnf.
-    constructors. applys term_abs L. intros x Hx. forwards*: M x. }
-  { introv HV1 M1 M2. forwards V1: value_of_not_var M1 HV1.
-    inverts V1; inverts M1. tests C: (value t2).
-    { applys* coomnibig_beta. applys* IH. pick_fresh x.
-      rewrite* (@subst_intro x). apply_empty* typing_subst. }
-    { applys* coomnibig_app_2 (post Y T1).
-      { applys* IH. hnfs*. }
-      { introv (Y'&EY'&HY'&HT'). applys* IH. applys himpl_trans HQ.
-        applys post_extends EY'. } } }
+  { intros L M. asserts Wf1: (term (trm_abs t1)).
+    { applys term_abs L. intros x Hx. forwards*: M x. }
+    applys* coomnibig_val. { simple*. }{ applys* HQ. } }
+  { introv Ht1 Ht2. tests V1: (value t1).
+    { tests V2: (value t2).
+      { inverts V1; inverts Ht1.
+        applys* coomnibig_beta. applys* IH. pick_fresh x.
+        rewrite* (@subst_intro x). apply_empty* typing_subst. }
+      { sound_ctx coomnibig_app_2. } }
+    { sound_ctx coomnibig_app_1. } }
   { intros K. applys* coomnibig_val. }
-  { intros K. applys* coomnibig_val. }
-  { intros K B. applys* coomnibig_val. }
-  { intros HV1 M1. forwards V1: value_of_not_var M1 HV1.
-    applys* coomnibig_ref.
-    { intros l Hl. applys HQ. applys* post_ref. } }
-  { introv HV1 M1. forwards V1: value_of_not_var M1 HV1.
-    inverts V1; inverts M1.
-    destruct~ ((proj33 HS) l0 T) as [t [Hast Typt]].
-    applys* coomnibig_get. }
-  { introv HV1 HV2 M1 M2. forwards V2: value_of_not_var M2 HV2.
-    forwards V1: value_of_not_var M1 HV1. inverts V1; inverts M1.
-    applys* coomnibig_set. applys HQ. applys* post_set. }
-  { introv HV1 M1. forwards V1: value_of_not_var M1 HV1.
-     inverts V1; inverts M1. applys* coomnibig_rand.
-     (* details: intros. applys HQ. unfolds. exists Y. splits*. *)  }
+  { intros K. applys* coomnibig_val. simple*. }
+  { intros K B. applys* coomnibig_val. simple*. }
+  { introv Ht1. tests V1: (value t1).
+    { applys* coomnibig_ref. intros l Hl. applys HQ.
+      exists (Y & l ~ T0). lets: (proj32 HS) Hl. splits*.
+      { applys* sto_typing_push. } }
+    { sound_ctx coomnibig_ref_1. } }
+  { introv Ht1. tests V1: (value t1).
+    { inverts V1; inverts Ht1. forwards (r&Vr&Hr&Tr): (proj33 HS) l0.
+      { eauto.  } applys* coomnibig_get. }
+    { sound_ctx coomnibig_get_1. } }
+  { introv Ht1 Ht2. tests V1: (value t1).
+    { tests V2: (value t2).
+      { inverts V1; inverts Ht1. forwards (r&Vr&Hr&Tr): (proj33 HS) l0.
+        { eauto. } applys* coomnibig_set. applys HQ.
+        exists Y. destruct HS as [StoOk [Dom Map]]. splits*.
+        { splits*. intros l T' HB. tests: (l = l0).
+          { exists t2. rewrites* (>> binds_functional T' T0 HB). }
+          { destruct (Map _ _ HB) as (t'&Val&Has&Typ). exists* t'. } } }
+      { sound_ctx coomnibig_set_2. } }
+    { sound_ctx coomnibig_set_1. } }
+  { introv Ht1. tests V1: (value t1).
+    { inverts V1; inverts Ht1. applys* coomnibig_rand. }
+    { sound_ctx (>> coomnibig_rand_1 (post Y typ_int)). } }
 Qed.
-
-(** The original statement is a trivial consequence. *)
-
-Lemma coomnibig_soundness_result : forall t mu Y T,
-  Y |== mu ->
-  empty ! Y |= t ~: T ->
-  coomnibig (t,mu) (post Y T).
-Proof using.
-  introv HS HT. applys* coomnibig_soundness_coinduction. hnfs*.
-Qed.
-
-(** Note that the statement over which we carried the coinduction
-    is equivalent, not stronger. *)
-
-Lemma coomnibig_soundness_coinduction' :
-  coomnibig_soundness.
-Proof using.
-  unfolds. introv HS HT HQ. applys coomnibig_conseq.
-  { applys* coomnibig_soundness_result. }
-  { auto. }
-Qed.
-
-(** We next give a generic proof that [omnibig_soundness_coinduction]
-    entails [type soundness]. *)
-
-(** In the file Omnisemantics.v, we proved in lemma [safe_of_coomnibig] that
-    [coomnibig c Q] for any [Q] entails [safe Q], for a coinductive-big-step
-    definition of safety, which we proved equivalent to the small-step
-    characterization of safety used in the present file (lemma [ssafe_eq_safe]).
-    To avoid reproducing all the development here, let us simply assume in
-    this file the property [safe_of_coomnibig]. *)
-
-Parameter safe_of_coomnibig : forall c Q,
-  coomnibig c Q ->
-  safe c.
-
-(** We show that the result established by coinduction indeed
-    entails type soundess. *)
-
-Lemma soundness_of_coomnibig_soundness :
-  coomnibig_soundness ->
-  type_soundness.
-Proof using.
-  intros HS (t,mu) (Y&T&HY&HT). applys* safe_of_coomnibig.
-  applys* coomnibig_soundness_result.
-Qed.
-
 
