ln/STLC_Ref_Soundness_Common.v
@@ -1,0 +1,85 @@
+(***************************************************************************
+* Safety for STLC with References - Common Parts of Type Soundness Proofs  *
+* Arthur Chargueraud, Dec 2023                                             *
+***************************************************************************)
+
+Set Implicit Arguments.
+Require Export STLC_Ref_Definitions STLC_Ref_Infrastructure.
+
+Hint Constructors typing.
+
+(** Typing is preserved by weakening. *)
+
+Lemma typing_weaken : forall G E F Y t T,
+   (E & G) ! Y |= t ~: T ->
+   ok (E & F & G) ->
+   (E & F & G) ! Y |= t ~: T.
+Proof.
+  introv Typ. gen_eq H: (E & G). gen G.
+  induction Typ; introv EQ Ok; subst.
+  apply* typing_var. apply* binds_weaken.
+  apply_fresh* typing_abs as y. apply_ih_bind* H0.
+  autos*.
+  autos*.
+  autos*.
+  autos*.
+  autos*.
+  autos*.
+  autos*.
+  autos*.
+Qed.
+
+(** Typing is preserved by substitution. *)
+
+Lemma typing_subst : forall F E Y t T z u U,
+  (E & z ~ U & F) ! Y |= t ~: T ->
+  E ! Y |= u ~: U ->
+  (E & F) ! Y |= [z ~> u]t ~: T.
+Proof.
+  introv Typt Typu. gen_eq G: (E & z ~ U & F). gen F.
+  induction Typt; introv Equ; subst; simpl subst.
+  case_var.
+    binds_get H0. apply_empty* typing_weaken.
+    binds_cases H0; apply* typing_var.
+  apply_fresh typing_abs as y.
+   rewrite* subst_open_var. apply_ih_bind* H0.
+  autos*.
+  autos*.
+  autos*.
+  autos*.
+  autos*.
+  autos*.
+  autos*.
+  autos*.
+Qed.
+
+(** Typing is preserved by an extension of store typing. *)
+
+Lemma typing_stability : forall Y E Y' t T,
+  E ! Y |= t ~: T ->
+  extends Y Y' ->
+  E ! Y' |= t ~: T.
+Proof.
+  introv Typ Ext. induction* Typ.
+Qed.
+
+Hint Resolve typing_stability.
+
+(** Store typing preserved by allocation of a well-typed term. *)
+
+Lemma sto_typing_push : forall Y mu l t T,
+  Y |== mu ->
+  value t ->
+  empty ! Y |= t ~: T ->
+  l # mu -> l # Y ->
+  (Y & l ~ T) |== (mu & l ~ t).
+Proof.
+  unfold sto_typing. introv (StoOk&Dom&Ext). splits 3.
+    auto.
+    intros l0 Fr. simpl_dom. lets: (Dom l0).
+      asserts* Fr2: (l <> l0). asserts* Fr3: (l0 # Y). auto.
+    intros l' T' Has. binds_cases Has.
+      destruct (Ext _ _ B) as (t'&Hast'&Typt').
+       exists* t'.
+      subst. exists* t.
+Qed.
