ln/STLC_Ref_Soundness_OmniSmall.v
@@ -1,0 +1,187 @@
+(***************************************************************************
+* Safety for STLC with References - Proof in Omni-Small-Step               *
+* Arthur Chargueraud, Dec 2023                                             *
+***************************************************************************)
+
+(** The proof is explained in the Omni-Semantics paper (TOPLAS'23).
+     http://www.chargueraud.org/research/2022/omnisemantics/omnisemantics.pdf *)
+
+Set Implicit Arguments.
+Require Import STLC_Ref_Soundness_Common.
+
+
+(* ********************************************************************** *)
+(** * Definition of Omni-Small-Step Semantics *)
+
+(** The omni-small-step judgment [omnismall c P], where [P] is a postcondition,
+    asserts that [c] is not stuck and that in one step it reaches a configuration
+    that satisfies [P]. *)
+
+CoInductive omnismall : conf -> (conf->Prop) -> Prop :=
+  | omnismall_beta : forall mu t1 t2 P,
+      sto_ok mu ->
+      term (trm_abs t1) ->
+      value t2 ->
+      P (t1 ^^ t2, mu) ->
+      omnismall (trm_app (trm_abs t1) t2, mu) P
+  | omnismall_ref : forall mu t1 P,
+      sto_ok mu ->
+      value t1 ->
+      (forall l, l # mu -> P (trm_loc l, (mu & l ~ t1))) ->
+      omnismall (trm_ref t1, mu) P
+  | omnismall_get : forall mu l t P,
+      sto_ok mu ->
+      binds l t mu ->
+      P (t, mu) ->
+      omnismall (trm_get (trm_loc l), mu) P
+  | omnismall_set : forall mu l t2 P,
+      sto_ok mu ->
+      value t2 ->
+      P (trm_unit, mu & l ~ t2) ->
+      omnismall (trm_set (trm_loc l) t2, mu) P
+  | omnismall_rand : forall mu n P,
+      (forall m, 0 <= m < max n 1 -> P ((trm_int m), mu)) ->
+      omnismall (trm_rand (trm_int n), mu) P
+
+  | omnismall_app_1 : forall mu t1 t2 P1 P,
+      omnismall (t1, mu) P1 ->
+      (forall t1' mu', P1 (t1',mu') -> P (trm_app t1' t2, mu')) ->
+      omnismall (trm_app t1 t2, mu) P
+  | omnismall_app_2 : forall mu t1 t2 P1 P,
+      value t1 ->
+      omnismall (t2, mu) P1 ->
+      (forall t2' mu', P1 (t2',mu') -> P (trm_app t1 t2', mu')) ->
+      omnismall (trm_app t1 t2, mu) P
+  | omnismall_ref_1 : forall mu t1 P1 P,
+      omnismall (t1, mu) P1 ->
+      (forall t1' mu', P1 (t1',mu') -> P (trm_ref t1', mu')) ->
+      omnismall (trm_ref t1, mu) P
+  | omnismall_get_1 : forall mu t1 P1 P,
+      omnismall (t1, mu) P1 ->
+      (forall t1' mu', P1 (t1',mu') -> P (trm_get t1', mu')) ->
+      omnismall (trm_get t1, mu) P
+  | omnismall_set_1 : forall mu t1 t2 P1 P,
+      omnismall (t1, mu) P1 ->
+      (forall t1' mu', P1 (t1',mu') -> P (trm_set t1' t2, mu')) ->
+      omnismall (trm_set t1 t2, mu) P
+  | omnismall_set_2 : forall mu t1 t2 P1 P,
+      value t1 ->
+      omnismall (t2, mu) P1 ->
+      (forall t2' mu', P1 (t2',mu') -> P (trm_set t1 t2', mu')) ->
+      omnismall (trm_set t1 t2, mu) P
+  | omnismall_rand_1 : forall mu t1 P1 P,
+      omnismall (t1, mu) P1 ->
+      (forall t1' mu', P1 (t1',mu') -> P (trm_rand t1', mu')) ->
+      omnismall (trm_rand t1, mu) P.
+
+(** The definition above may be considered as the reference semantics,
+    in replacement of the standard small-step judgment [c --> c'].
+    The folder '/omni' of this repository contains a proof of the
+    following equivalence between small-step and omni-small-step. *)
+
+Parameter omnismall_equiv_red : forall c P,
+  omnismall c P <->
+    (   (exists c', c --> c')
+     /\ (forall c', c --> c' -> P c')).
+
+
+(* ********************************************************************** *)
+(** * Statement *)
+
+(** Postcondition associated with a well-typed configuration *)
+
+Definition post (Y:phi) (T:typ) : conf->Prop :=
+  fun '(t,mu) =>
+    exists Y', extends Y Y'
+             /\ Y' |== mu
+             /\ empty ! Y' |= t ~: T.
+
+(** Goal is to prove omnismall-soundness: well typed configurations
+    are either made of a value or can take a step towards a configuration
+    that satisfies the same type, for an extended store typing. *)
+
+Definition omnismall_soundness := forall mu t Y T,
+  Y |== mu ->
+  empty ! Y |= t ~: T ->
+  value t \/ omnismall (t,mu) (post Y T).
+
+
+(* ********************************************************************** *)
+(** * Soundness proof *)
+
+Lemma post_current : forall Y mu t T,
+  Y |== mu ->
+  empty ! Y |= t ~: T ->
+  post Y T (t,mu).
+Proof using.
+  introv HS HT. exists Y. splits*.
+Qed.
+
+Hint Resolve post_current.
+Hint Constructors typing.
+
+Ltac sound_ctx E := (* tactic for evaluation under context *)
+  let Y' := fresh "Y'" in
+  applys* E; try (introv (Y'&?&?&?); exists* Y').
+
+Lemma omnismall_soundness_result :
+  omnismall_soundness.
+Proof using.
+  introv HS HT. gen_eq E: (@empty typ). gen mu.
+  induction HT; intros; subst; try solve [left* ].
+  { false* binds_empty_inv. }
+  { left*. constructors.
+    { applys term_abs L. intros x Hx. forwards*: H x. } }
+  { right. forwards* [Val1|HR1]: IHHT1.
+    { forwards* [Val2|HR2]: IHHT2.
+      { inversions HT1; inversions Val1. applys* omnismall_beta.
+        { applys* post_current.
+          pick_fresh x. rewrite* (@subst_intro x).
+          apply_empty* typing_subst. } }
+      { sound_ctx omnismall_app_2. } }
+    { sound_ctx omnismall_app_1. } }
+  { right. forwards* [Val1|HR1]: IHHT.
+    { applys* omnismall_ref. intros l Hl. exists (Y & l ~ T).
+      lets: (proj32 HS) Hl. splits*. { applys* sto_typing_push. } }
+    { sound_ctx omnismall_ref_1. } }
+  { right. forwards* [Val1|HR1]: IHHT.
+    { inverts HT; inverts Val1. destruct~ ((proj33 HS) l0 T) as (t&Valt&Hast&Typt).
+      applys* omnismall_get. }
+    { sound_ctx omnismall_get_1. } }
+  { right. forwards* [Val1|HR1]: IHHT1.
+    { forwards* [Val2|HR2]: IHHT2.
+      { inverts HT1; inverts Val1. destruct~ ((proj33 HS) l0 T) as (t&Valt&Hast&Typt).
+        applys* omnismall_set. exists Y.
+        destruct HS as (StoOk&Dom&Map). splits*.
+        { splits*. intros l T' HB. tests: (l = l0).
+          { exists t2. rewrites* (>> binds_functional T' T HB). }
+          { destruct (Map _ _ HB) as (t'&Has&Typ). exists* t'. } } }
+      { sound_ctx omnismall_set_2. } }
+    { sound_ctx omnismall_set_1. } }
+  { right. forwards* [Val1|HR1]: IHHT.
+    { inverts HT; inverts Val1. applys* omnismall_rand. }
+    { sound_ctx omnismall_rand_1. } }
+Qed.
+
+
+(* ********************************************************************** *)
+(** * Generic result: type soundness follows from omnismall-soudness *)
+
+(** We next give a generic proof that [omnismall_soundness_induction]
+    entails [type soundness] *)
+
+Lemma soundness_of_omnismall_soundness :
+  omnismall_soundness ->
+  soundness.
+Proof using.
+  introv Sou. intros (t,mu) (Y&T&HT&HY). introv HR.
+  gen_eq c: (t,mu). gen t mu Y T. induction HR; intros; subst.
+  { intros. forwards [HV|M]: Sou HY HT.
+    { left*. }
+    { right. rewrite* omnismall_equiv_red in M. } }
+  { lets [HV|M]: Sou HY HT.
+    { inverts HV; inverts H. }
+    { rewrite omnismall_equiv_red in M. destruct M as (M1&M2).
+      specializes M2 H. destruct c2 as (t2,mu2).
+      destruct M2 as (Y'&EY'&HY'&HT'). applys* IHHR HT'. } }
+Qed.
