ln/STLC_Ref_Soundness_Small.v
@@ -4,8 +4,8 @@
 ***************************************************************************)
 
 Set Implicit Arguments.
-From TLC Require Import LibLN LibNat.
-Require Import STLC_Ref_Definitions STLC_Ref_Infrastructure.
+From TLC Require Import LibNat.
+Require Import STLC_Ref_Soundness_Common.
 
 
 (* ********************************************************************** *)
@@ -32,83 +32,6 @@ Definition progress := forall Y t mu T,
 (* ********************************************************************** *)
 (** * Proofs *)
 
-Hint Constructors typing.
-
-(** Typing is preserved by weakening. *)
-
-Lemma typing_weaken : forall G E F Y t T,
-   (E & G) ! Y |= t ~: T ->
-   ok (E & F & G) ->
-   (E & F & G) ! Y |= t ~: T.
-Proof.
-  introv Typ. gen_eq H: (E & G). gen G.
-  induction Typ; introv EQ Ok; subst.
-  apply* typing_var. apply* binds_weaken.
-  apply_fresh* typing_abs as y. apply_ih_bind* H0.
-  autos*.
-  autos*.
-  autos*.
-  autos*.
-  autos*.
-  autos*.
-  autos*.
-  autos*.
-Qed.
-
-(** Typing is preserved by substitution. *)
-
-Lemma typing_subst : forall F E Y t T z u U,
-  (E & z ~ U & F) ! Y |= t ~: T ->
-  E ! Y |= u ~: U ->
-  (E & F) ! Y |= [z ~> u]t ~: T.
-Proof.
-  introv Typt Typu. gen_eq G: (E & z ~ U & F). gen F.
-  induction Typt; introv Equ; subst; simpl subst.
-  case_var.
-    binds_get H0. apply_empty* typing_weaken.
-    binds_cases H0; apply* typing_var.
-  apply_fresh typing_abs as y.
-   rewrite* subst_open_var. apply_ih_bind* H0.
-  autos*.
-  autos*.
-  autos*.
-  autos*.
-  autos*.
-  autos*.
-  autos*.
-  autos*.
-Qed.
-
-(** Typing is preserved by an extension of store typing. *)
-
-Lemma typing_stability : forall Y E Y' t T,
-  E ! Y |= t ~: T ->
-  extends Y Y' ->
-  E ! Y' |= t ~: T.
-Proof.
-  introv Typ Ext. induction* Typ.
-Qed.
-
-Hint Resolve typing_stability.
-
-(** Store typing preserved by allocation of a well-typed term. *)
-
-Lemma sto_typing_push : forall Y mu l t T,
-  Y |== mu ->
-  empty ! Y |= t ~: T ->
-  l # mu -> l # Y ->
-  (Y & l ~ T) |== (mu & l ~ t).
-Proof.
-  unfold sto_typing. introv [StoOk [Dom Ext]]. splits 3.
-    auto.
-    intros l0 Fr. simpl_dom. lets: (Dom l0).
-      asserts* Fr2: (l <> l0). asserts* Fr3: (l0 # Y). auto.
-    intros l' T' Has. binds_cases Has.
-      destruct (Ext _ _ B) as [t' [Hast' Typt']].
-       exists* t'.
-      subst. exists* t.
-Qed.
-
 (** A simple short-hand to help clarifying the following proof.
   It simply destruct the induction hypothesis into smaller pieces. *)
 
@@ -118,7 +41,7 @@ Ltac pres H t' mu' :=
   let Typt' := fresh "Typt'" in
   let TypSto' := fresh "TypSto'" in
   destruct~ (H (@refl_equal env empty) t' mu')
-                  as [Y' [Ext [Typt' TypSto']]].
+                  as (Y'&Ext&Typt'&TypSto').
 
 (** Preservation (typing is preserved by reduction). *)
 
@@ -138,14 +61,14 @@ Proof.
   pres IHTyp t1' mu'. exists* Y'.
   exists Y. splits~ 3.
     inversions Typ.
-     destruct~ ((proj33 TypSto) l T) as [t [Hast Typt]].
+     destruct~ ((proj33 TypSto) l T) as (t&Valt&Hast&Typt).
      rewrite~ (binds_functional H4 Hast).
   pres IHTyp t1' mu'. exists* Y'.
   exists Y. inversions Typ1. splits~ 3.
-    destruct TypSto as [StoOk [Dom Map]]. splits~ 3.
+    destruct TypSto as (StoOk&Dom&Map). splits~ 3.
      intros. tests: (l = l0).
        exists t2. split~. rewrite~ (binds_functional H H6).
-       destruct (Map _ _ H) as [t [Has Typ]]. exists* t.
+       destruct (Map _ _ H) as (t&Has&Typ). exists* t.
   pres IHTyp1 t1' mu'. exists* Y'.
   pres IHTyp2 t2' mu'. exists* Y'.
   exists* Y.
@@ -161,35 +84,40 @@ Proof.
   induction Typ; intros; subst.
   false* binds_empty_inv.
   left*.
-  right. destruct~ IHTyp1 as [Val1 | [t1' [mu' Red1]]].
-    destruct~ IHTyp2 as [Val2 | [t2' [mu' Red2]]].
+  right. destruct~ IHTyp1 as [Val1 | (t1'&mu'&Red1)].
+    destruct~ IHTyp2 as [Val2 | (t2'&mu'&Red2)].
       inversions Typ1; inversions Val1. exists* (t0 ^^ t2) mu.
       exists* (trm_app t1 t2') mu'.
     exists* (trm_app t1' t2).
   left*.
   left*.
   left*.
-  right. destruct~ IHTyp as [Val1 | [t1' [mu' Red1]]].
+  right. destruct~ IHTyp as [Val1 | (t1'&mu'&Red1)].
     destruct (var_fresh (dom mu)) as [l Fr].
      exists* (trm_loc l) (mu & l ~ t1).
     exists* (trm_ref t1') mu'.
-  right. destruct~ IHTyp as [Val1 | [t1' [mu' Red1]]].
+  right. destruct~ IHTyp as [Val1 | (t1'&mu'&Red1)].
     inversions Val1; inversions Typ.
-     destruct ((proj33 H) _ _ H5) as [t' [Has' Typt']].
+     destruct ((proj33 H) _ _ H5) as (t'&Has'&Typt').
      exists* t' mu.
     exists* (trm_get t1') mu'.
-  right. destruct~ IHTyp1 as [Val1 | [t1' [mu' Red1]]].
+  right. destruct~ IHTyp1 as [Val1 | (t1'&mu'&Red1)].
     destruct~ IHTyp2 as [Val2 | [t2' [mu' Red2]]].
       inversions Val1; inversions Typ1.
-       destruct ((proj33 H) _ _ H5) as [t' [Has' Typt']].
+       destruct ((proj33 H) _ _ H5) as (t'&Has'&Typt').
        exists* trm_unit (mu & l ~ t2).
       exists* (trm_set t1 t2') mu'.
     exists* (trm_set t1' t2) mu'.
-  right. destruct~ IHTyp as [Val1 | [t1' [mu' Red1]]].
+  right. destruct~ IHTyp as [Val1 | (t1'&mu'&Red1)].
     inversions Val1; inversions Typ.
-     exists* (trm_int 0) mu. constructors*. lia.
+     exists* (trm_int 0) mu. constructors*.
+       unfold max. case_if; nat_math.
     exists* (trm_rand t1') mu'.
 Qed.
+
+
+(* ********************************************************************** *)
+(** * Generic result: type soundness follows from preservation and progress *)
 
 (** Type soundness (well-typed configurations can only reach
     safe configurations, i.e. configurations that are values
